A12Kernel.lean
@@ -192,6 +192,7 @@ import A12Kernel.Elaboration.AddressedDateRangeBoundPart
 import A12Kernel.Elaboration.AddressedNumberField
 import A12Kernel.Elaboration.CurrentRepetitionComputation
 import A12Kernel.Elaboration.CurrentRepetitionNumberToString
+import A12Kernel.Elaboration.CurrentRepetitionNumberToStringRelation
 import A12Kernel.Elaboration.CurrentRepetitionStringToNumber
 import A12Kernel.Elaboration.CurrentRepetitionAlternatingChain
 import A12Kernel.Elaboration.RepeatableNumberAggregateCascade
